Added with-global-stobj.
Quoting :DOC note-8-5:

  A new macro, with-global-stobj, allows reading and writing of a
  [stobj] in the body of a function without having to pass it as a
  formal parameter, by accessing the stobj from the ACL2 [state].
  See with-global-stobj.  Thanks to Rob Sumners and Sol Swords for
  requesting this feature (originally, to support a global
  [stobj-table]) and for helpful discussions about its design.

An example of how with-global-stobj might be employed to implement a
global stobj-table may be found in
books/system/tests/with-global-stobj-input.lsp; see "Global
stobj-table".

doc.lisp
@@ -4280,6 +4280,9 @@ Subtopics
       (with-fast-alist name form) causes name to be a fast alist for the
       execution of form.
 
+  [With-global-stobj]
+      Operate on a global single-threaded object
+
   [With-guard-checking]
       Suppress or enable guard-checking for a form
 
@@ -23868,6 +23871,12 @@ Miscellaneous Remarks, with discussion of possible user errors.
                        (not (h t))))
      :PASSED
     ACL2 !>
+
+  The advanced feature, [with-global-stobj], imposes certain
+  restrictions on a defattach event.  You can probably ignore this
+  point unless you get an error pertaining to with-global-stobj.  For
+  relevant documentation see [with-global-stobj], specifically the
+  section on ``Constrained Functions and Defattach''.
 
   We conclude with an example promised above, showing why it is
   necessary in general to unattach all function symbols in an
@@ -64886,8 +64895,9 @@ Subtopics
   [never-memoize]; or if it is excluded because it is ``special'' in
   the sense that it is in the \"COMMON-LISP\" [package], it has no
   fixed output signature (i.e., it is in the value of the list
-  constant (if return-last do$), (if return-last do$)), it has
-  associated raw-Lisp code, or it is used in the implementation of
+  constant (if return-last do$ read-user-stobj-alist), (if
+  return-last do$ read-user-stobj-alist)), it has associated raw-Lisp
+  code, or it is used in the implementation of
   [hons-and-memoization].  A constrained function (typically, one
   that is introduced in the signature of an [encapsulate] event)
   cannot be memoized; in that case, one may wish to memoize its
@@ -91074,6 +91084,13 @@ New Features
   outside the prover.  Thanks to Sol Swords for requesting such a
   utility.
 
+  A new macro, [with-global-stobj], allows reading and writing of a
+  [stobj] in the body of a function without having to pass it as a
+  formal parameter, by accessing the stobj from the ACL2 [state].
+  See [with-global-stobj].  Thanks to Rob Sumners and Sol Swords for
+  requesting this feature (originally, to support a global
+  [stobj-table]) and for helpful discussions about its design.
+
 
 Heuristic and Efficiency Improvements
 
@@ -115317,22 +115334,22 @@ Subtopics
   a [keyword-value-listp], i.e., an alternating list of keywords and
   values starting with a keyword.  In this case ((fn x1 ... xn) =>
   val) must be a legal signature as described above.  The legal
-  keywords in k are :GUARD and :FORMALS (except that for ACL2(r),
-  also see the remark about :CLASSICALP later in this topic).  The
-  value following :FORMALS is to be the list of formal parameters of
-  fn, which must be consistent with the parameters specified in (fn
-  x1 ... xn): they must both specify the same arity (number of formal
-  parameters) and the same [stobj] inputs.  The value following
-  :GUARD is a term that is to be the [guard] of fn.  Note that this
-  guard is never actually evaluated, and is not subject to the guard
-  verification performed on functions introduced by [defun] (see
-  [verify-guards]).  Said differently: this guard need not itself
-  have a guard of t.  Indeed, the guard is only used for attachments;
-  see [defattach].  Note that if :GUARD is supplied, then :FORMALS
-  must also be supplied as a list of distinct variables that includes
-  all variables occurring free in the specified guard.  One final
-  observation about guards: if the :GUARD keyword is omitted, then
-  the guard defaults to T.
+  keywords in k are normally :GUARD and :FORMALS (but see remarks at
+  the end of this topic regarding :GLOBAL-STOBJS and, for ACL2(r),
+  :CLASSICALP).  The value following :FORMALS is to be the list of
+  formal parameters of fn, which must be consistent with the
+  parameters specified in (fn x1 ... xn): they must both specify the
+  same arity (number of formal parameters) and the same [stobj]
+  inputs.  The value following :GUARD is a term that is to be the
+  [guard] of fn.  Note that this guard is never actually evaluated,
+  and is not subject to the guard verification performed on functions
+  introduced by [defun] (see [verify-guards]).  Said differently:
+  this guard need not itself have a guard of t.  Indeed, the guard is
+  only used for attachments; see [defattach].  Note that if :GUARD is
+  supplied, then :FORMALS must also be supplied as a list of distinct
+  variables that includes all variables occurring free in the
+  specified guard.  One final observation about guards: if the :GUARD
+  keyword is omitted, then the guard defaults to T.
 
   Before ACL2 supported user-declared single-threaded objects there was
   only one single-threaded object: ACL2's built-in notion of [state].
@@ -115369,9 +115386,12 @@ Subtopics
   or else is a list of such names.  Every name in names must have
   been previously defined as a stobj via [defstobj] or [defabsstobj].
 
-  As promised above, we conclude with a remark about an additional
-  keyword, :CLASSICALP, that is legal for ACL2(r) (see [real]).  The
-  value of this keyword must be t (the default) or nil, indicating
+  As promised above, we conclude with a remark about additional
+  keywords.  The keyword :GLOBAL-STOBJS specifies the use of the
+  macro, with-global-stobj, in attachments (see [defattach]); see
+  [with-global-stobj] for explanation of this keyword.  The keyword
+  :CLASSICALP is legal for ACL2(r) only (see [real]).  The value of
+  this keyword must be t (the default) or nil, indicating
   respectively whether fn is classical or not.")
  (SIGNED-BYTE-P
   (NUMBERS ACL2-BUILT-INS)
@@ -117126,6 +117146,9 @@ Subtopics
   [User-stobjs-modified-warnings]
       Interactions of [trans-eval] with [stobj]s that violate applicative
       semantics
+
+  [With-global-stobj]
+      Operate on a global single-threaded object
 
   [With-local-state]
       Locally bind state
@@ -120439,8 +120462,8 @@ List of a few built-in system utilities
       function is make-lambda-application, but that one drops unused
       formals, while make-lambda-term does not.
     * (maybe-convert-to-mv uterm): Given the untranslated [term] uterm,
-      replace each of its top-level calls of [list] by a call oof
-      [mv] on the same arguments.
+      replace each of its top-level calls of [list] by a call of [mv]
+      on the same arguments.
     * (nvariablep x): For a [pseudo-termp] x, return true iff x is not a
       variable (i.e. it is a quoted constant or a function call).
     * (partition-rest-and-keyword-args x keys): x should be a list of the
@@ -120496,8 +120519,8 @@ List of a few built-in system utilities
       Note that fn must be a symbol, not a [lambda] expression.
       Moreover fn must not be a member of the list value of the
       constant *stobjs-out-invalid*, i.e., the list (if return-last
-      do$), since for these functions arbitrary multiple values may
-      be returned.
+      do$ read-user-stobj-alist), since for these functions arbitrary
+      multiple values may be returned.
     * (subcor-var vars terms form): For a list vars of symbols, a list
       terms of [pseudo-termp]s, and a [pseudo-termp] form,
       substitute, in form, the i-th variable from vars with the i-th
@@ -125551,6 +125574,10 @@ Subtopics
   normally results in no additional output.  (For details about
   ``caused an error'', see the definition of top-level in the ACL2
   source code, and see [ld-error-action].)
+
+  Since the defined function top-level takes only state as a parameter,
+  the given form should not include any user-defined [stobj]s that
+  occur free in the form.
 
   Finally, note that since top-level runs a function that is defined in
   :[program] mode, it is possible for a raw lisp error to occur.
@@ -134732,6 +134759,595 @@ Concluding Remark
   Note that with-fast-alist will cause logically tail-recursive
   functions not to execute tail-recursively if its cleanup phase
   happens after the tail-recursive call returns.")
+ (WITH-GLOBAL-STOBJ
+  (STOBJ ACL2-BUILT-INS)
+  "Operate on a global single-threaded object
+
+  See [stobj] for an introduction to single-threaded objects.  Also see
+  [defstobj] for additional background.
+
+  The with-global-stobj macro is a relatively advanced utility that
+  allows stobjs to be accessed directly from the ACL2 [state].
+  Examples may be found in [community-book] file
+  books/system/tests/with-global-stobj-input.lsp; we draw heavily
+  from them below.
+
+    Example Forms:
+
+    ; Read-only form (length 3)
+    (with-global-stobj st
+      (fld st))
+
+    ; Updating form (length 4; (returns state))
+    (with-global-stobj
+      st ; bound stobj
+      (st) ; output signature of body
+      ;; body:
+      (update-fld x st))
+
+    ; Updating form (length 4; returns (mv * * state st2))
+    (with-global-stobj
+      st ; bound stobj
+      (nil st nil state st2) ; output signature of body
+      ;; body:
+      (let* ((st (update-fld x st))
+             (st2 (update-fld2 x st2)))
+        (mv (fld st) st (fld st2) state st2)))
+
+  In the forms above, we call st the stobj that is ``bound by'' the
+  with-global-stobj call.  Each updating form specifies an output
+  signature as a list, which must contain the stobj bound by the
+  form, whose elements are all nil (designating a non-stobj value) or
+  a stobj name.  That output signature reflects the result of the
+  body; the entire form does not return the bound stobj, but does
+  return [state], as explained below.
+
+  With-global-stobj is a macro, and the example forms above expand as
+  follows.
+
+    ACL2 !>:trans1 (with-global-stobj st
+                     (fld st))
+     (LET ((ST (READ-USER-STOBJ-ALIST 'ST STATE)))
+          (FLD ST))
+    ACL2 !>:trans1 (with-global-stobj st
+                     (st)
+                     (update-fld x st))
+     (LET ((ST (READ-USER-STOBJ-ALIST 'ST STATE)))
+          (LET ((ST (UPDATE-FLD X ST)))
+               (WRITE-USER-STOBJ-ALIST 'ST ST STATE)))
+    ACL2 !>:trans1 (with-global-stobj st
+                     (nil st nil state st2)
+                     (let* ((st (update-fld x st))
+                            (st2 (update-fld2 x st2)))
+                       (mv (fld st) st (fld st2) state st2)))
+     (LET ((ST (READ-USER-STOBJ-ALIST 'ST STATE)))
+          (MV-LET ({WGS}0 ST {WGS}1 STATE ST2)
+                  (LET* ((ST (UPDATE-FLD X ST))
+                         (ST2 (UPDATE-FLD2 X ST2)))
+                        (MV (FLD ST) ST (FLD ST2) STATE ST2))
+                  (LET ((STATE (WRITE-USER-STOBJ-ALIST 'ST ST STATE)))
+                       (MV? {WGS}0 {WGS}1 STATE ST2))))
+    ACL2 !>
+
+  The first illustrates that in the read-only form, the bound stobj,
+  which is st in that example, is bound to its value in the
+  user-stobj-alist field of the ACL2 [state].  The second and third
+  similarly bind the stobj, st, but then update that stobj according
+  to the body of the with-global-stobj call (its last argument) and
+  then update the user-stobj-alist of the state with that stobj's
+  resulting value.  You can of course use :[trans1] in this way to
+  see expansions of other with-global-stobj calls.
+
+  Note that ACL2 expects you to use with-global-stobj, not its
+  expansions in terms of the [non-executable] functions
+  read-user-stobj-alist, which accesses the bound stobj from the
+  user-stobj-alist of state, and write-user-stobj-alist, which
+  completes the write for updating with-global-stobj forms.  These
+  are defined as follows, in terms of the ACL2 state's
+  user-stobj-alist field, which maps stobj names to their values.
+
+    (defun-nx read-user-stobj-alist (st state)
+      (declare (xargs :guard (symbolp st)
+                      :stobjs state))
+      (cdr (assoc-eq st (user-stobj-alist1 state))))
+
+    (defun-nx write-user-stobj-alist (st val state)
+      (declare (xargs :guard (symbolp st)
+                      :stobjs state))
+      (update-user-stobj-alist1
+       (put-assoc-eq st val (user-stobj-alist1 state))
+       state))
+
+  With-global-stobj can be useful when you want a function to read or
+  write a stobj but you don't want to pass that stobj as a formal
+  parameter.  As long as you pass state as a formal parameter, you
+  can access the stobj using with-global-stobj.
+
+  This topic is intended to be sufficient preparation for the use of
+  with-global-stobj.  Those who want to read more about design and
+  underlying theory are welcome to peruse the (long) ACL2 source code
+  comments, ``Essay on the Design of With-global-stobj'' and ``Essay
+  on Correctness of Evaluation with Stobjs''.
+
+
+More Examples
+
+  As noted above, examples may be found in [community-book] file
+  books/system/tests/with-global-stobj-input.lsp.  Here we discuss
+  some of those examples.
+
+  Let us start by introducing a couple of stobjs.
+
+    (defstobj st fld)
+    (defstobj st2 fld2 :congruent-to st)
+
+  Calls of with-global-stobj are illegal at the top level (as opposed
+  to occurrences in the bodies of a definition or a theorem.
+
+    (with-global-stobj st (fld st))
+
+  One solution may be to use [top-level].
+
+    (top-level (with-global-stobj st (fld st)))
+
+  Normally, however, with-global-stobj is used inside definitions.
+  Here we read and write the stobj, st, directly from the ACL2
+  [state].
+
+    (defun rd0 (state)
+      (declare (xargs :stobjs state))
+      (with-global-stobj st (fld st)))
+
+    (defun wr0 (x state)
+      (declare (xargs :stobjs state))
+      (with-global-stobj st (st) (update-fld x st)))
+
+  Let's see these in action, first writing and then reading.
+
+    ACL2 !>(wr0 2 state)
+    <state>
+    ACL2 !>(rd0 state)
+    2
+    ACL2 !>(fld st)
+    2
+    ACL2 !>
+
+  We can use various stobj operations, even the rather fancy
+  [swap-stobjs], in the body of a with-global-stobj call.  The
+  following events are admissible.
+
+    (update-fld 1 st)
+    (update-fld 2 st2)
+
+    (defun f3 (st2 state)
+      (declare (xargs :stobjs (st2 state)))
+      (with-global-stobj
+        st
+        (st2 st)
+        (swap-stobjs st2 st)))
+
+    (f3 st2 state)
+
+    (assert-event (and (equal (fld st) 2)
+                       (equal (fld st2) 1)))
+
+  The following function writes to both st and st2 without passing in
+  either one (just state).  Notice that the inner with-global-stobj
+  call has a body that returns the indicated values st and st2, but
+  since st2 is bound by the call, it is dropped before returning from
+  the call, and state is added --- which explains the list (st state)
+  supplied to the outer call.
+
+    (defun write-global-st-st2 (fld fld2 state)
+      (declare (xargs :stobjs state))
+      (with-global-stobj st
+        (st state)
+        (let ((st (update-fld fld st)))
+          (with-global-stobj st2
+            (st st2)
+            (let ((st2 (update-fld fld2 st2)))
+              (mv st st2))))))
+
+  Let's check that this works as expected.
+
+    ACL2 !>(write-global-st-st2 'a 'b state)
+    <state>
+    ACL2 !>(fld st)
+    A
+    ACL2 !>(fld st2)
+    B
+    ACL2 !>
+
+  We can also read both fields.
+
+    (defun read-global-st-st2 (state)
+      (declare (xargs :stobjs state))
+      (with-global-stobj st
+        (with-global-stobj st2
+          (list (fld st) (fld st2)))))
+
+  Then, continuing with the session above:
+
+    ACL2 !>(read-global-st-st2 state)
+    (A B)
+    ACL2 !>
+
+  We can reason about with-global-stobj by reasoning about its
+  expansions.  Consider the following theorem (continuing the session
+  above).
+
+    (defthm rd0-of-wr0
+      (equal (rd0 (wr0 val state))
+             val))
+
+  This fails to prove, but each of the two checkpoints has a term of
+  the form (ASSOC-EQUAL 'ST (PUT-ASSOC-EQUAL 'ST _ _)).  That
+  suggests the following lemma.
+
+    (defthm assoc-equal-put-assoc-equal
+      (equal (assoc-equal key (put-assoc-equal key val alist))
+             (cons key val)))
+
+  This lemma proves automatically, after which rd0-of-wr0 proves
+  automatically.
+
+
+Syntax and Semantics
+
+  This section provides a reference for with-global-stobj.  The next
+  section discusses restrictions that avoid aliasing problems.
+
+    General Forms:
+    ; Read-only form (length 3):
+    (with-local-stobj st form)
+    ; Updating form (length 4):
+    (with-local-stobj st lst form)
+
+  where st is the name of a [stobj] that is user-defined (i.e., not
+  state), form is subject to syntactic restrictions discussed below,
+  and lst is a list, sometimes called an ``output signature''.  That
+  list indicates the list of N values returned by form, which must
+  include the bound stobj, st: thus lst is (st) if N is 1, indicating
+  that form returns an instance of that stobj; and otherwise form
+  returns multiple values (x0 x1 ... xk) where k is N-1 and for each
+  i, xi is either nil if the ith value is an ordinary value or else
+  is the name of a stobj returned in that position.
+
+  In each General Form above, st and form are called the ``bound
+  stobj'' and ``body'' of the with-local-stobj call (respectively).
+
+  For the updating form, the values actually returned are obtained by
+  removing st from lst and then, if state is not already in lst,
+  adding state at the end of lst.  Consider the following example.
+
+    (defun f0 (st2 state)
+      (declare (xargs :stobjs (st2 state)))
+      (with-global-stobj
+        st
+        (st st2 nil state)
+        (mv st st2 nil state)))
+
+  In this case, lst is (st st2 nil state), and the following expansion
+  shows that st has been dropped from the returned values.
+
+    ACL2 !>:trans1 (with-global-stobj
+                     st
+                     (st st2 nil state)
+                     (mv st st2 nil state))
+     (LET ((ST (READ-USER-STOBJ-ALIST 'ST STATE)))
+          (MV-LET (ST ST2 {WGS}0 STATE)
+                  (MV ST ST2 NIL STATE)
+                  (LET ((STATE (WRITE-USER-STOBJ-ALIST 'ST ST STATE)))
+                       (MV? ST2 {WGS}0 STATE))))
+    ACL2 !>
+
+  Evaluation of an updating with-global-stobj form always updates
+  state: specifically it updates its user-stobj-alist field (see
+  [state]).  The following example is similar to the one above,
+  except that this time the body of the with-global-stobj call does
+  not return state; nevertheless, the entire call does return state.
+  It illustrates that when state is not in the list given as the
+  second argument of a with-global-stobj call, then the
+  with-global-stobj form not only drops the bound stobj from its
+  return values but also adds state as the last returned value (or,
+  if the bound stobj was the sole symbol in the list, then the call
+  returns state).
+
+    ACL2 !>:trans1 (with-global-stobj
+                     st
+                     (st st2 nil)
+                     (mv st st2 nil))
+     (LET ((ST (READ-USER-STOBJ-ALIST 'ST STATE)))
+          (MV-LET (ST ST2 {WGS}0)
+                  (MV ST ST2 NIL)
+                  (LET ((STATE (WRITE-USER-STOBJ-ALIST 'ST ST STATE)))
+                       (MV? ST2 {WGS}0 STATE))))
+    ACL2 !>
+
+  Note that because with-global-stobj updates state, then state must be
+  a known stobj when with-global-stobj is called.  In particular, in
+  order to call with-global-stobj in the body of a function, state
+  should be a formal parameter of that function.
+
+
+Syntactic Restrictions to Avoid Aliasing
+
+  For the examples in this section, we continue to assume the following
+  stobj declarations.
+
+    (defstobj st fld)
+    (defstobj st2 fld2 :congruent-to st)
+
+  Consider the following definition.
+
+    (defun foo (st state)
+      (declare (xargs :stobjs (st state)))
+      (let ((state (with-global-stobj st
+                                      (st)
+                                      (update-fld 3 st))))
+        (mv (fld st) state)))
+
+  ACL2 admits that form, but causes an error with the following call of
+  foo.
+
+    ACL2 !>(foo st state)
+
+
+    ACL2 Error in TOP-LEVEL:  Illegal top-level form, (FOO ST STATE).
+    The stobj ST occurs free, yet may be bound by an updating WITH-GLOBAL-
+    STOBJ form, as the top-level form calls FOO, which makes an updating
+    WITH-GLOBAL-STOBJ call that binds ST.  See :DOC with-global-stobj.
+
+    ACL2 !>
+
+  Let us see why this call must be illegal; then we'll study the error
+  message.  The with-global-stobj form above will set the field, fld,
+  of st to the value, 3.  Moreover, ACL2 uses destructive update on
+  stobjs: the actual Lisp object representing st has value 3 in its
+  field, and this is the same object for which we return (fld st)
+  from foo.  So if (foo st state) were allowed to execute, it would
+  return the multiple values (3 <state>).  However, ACL2 can prove
+  that ACL2 returns (fld st) unchanged:
+
+    (thm (implies (stp st)
+                  (equal (mv-nth 0 (foo st state))
+                         (fld st))))
+
+  What we are seeing is a violation of single-threadedness.
+
+  Now let's look at the error message above.  It explains that ``the
+  stobj ST occurs free'' in (foo st state): indeed, st is the first
+  argument of that call.  Therefore, st can be accessed in that
+  top-level form; indeed, we have seen that it is returned as the
+  first value.  However, st can also be destructively modified
+  because of the updating with-global-stobj call in the body of foo:
+  ``the top-level form calls FOO, which makes an updating
+  WITH-GLOBAL-STOBJ call that binds ST.'' As we have discussed, that
+  updating call destroys single-threadedness, and hence must be
+  avoided.  We may call this an ``aliasing problem'', since the bound
+  stobj shares structure with the formal parameter.
+
+  By contrast, there is no such problem if we replace st by its
+  congruent stobj, st2, in the top-level call.
+
+    ACL2 !>(foo st2 state)
+    (NIL <state>)
+    ACL2 !>(fld st2)
+    NIL
+    ACL2 !>(fld st)
+    3
+    ACL2 !>
+
+  In this case there is no aliasing problem.  The formal parameter st
+  of foo is bound to the (global) value of st2, which does not share
+  structure with the (global) value of stobj st that is updated by
+  the with-global-stobj form.
+
+  Note that the aliasing problem can be buried through a chain of
+  function calls, as we now illustrate.  Function foo2 is like foo
+  above, with two changes: instead of updating the field with 3 we
+  update it with the formal parameter, val; and that update is done
+  inside the called function, foo2-sub, rather than directly in the
+  body of foo2.
+
+    (defun foo2-sub (val state)
+      (declare (xargs :stobjs state))
+      (with-global-stobj st
+                         (st)
+                         (update-fld val st)))
+
+    (defun foo2 (val st state)
+      (declare (xargs :stobjs (st state)))
+      (let ((state (foo2-sub val state)))
+        (mv (fld st) state val)))
+
+  The error message is essentially the same, except that the chain of
+  calls leading to the problematic updating with-global-stobj is
+  shown.  The behavior on st2 instead of st is fine, as before.
+
+    ACL2 !>(foo2 3 st state)
+
+
+    ACL2 Error in TOP-LEVEL:  Illegal top-level form, (FOO2 3 ST STATE).
+    The stobj ST occurs free, yet may be bound by an updating WITH-GLOBAL-
+    STOBJ form, as the top-level form calls FOO2, which calls FOO2-SUB,
+    which makes an updating WITH-GLOBAL-STOBJ call that binds ST.  See
+    :DOC with-global-stobj.
+
+    ACL2 !>(foo2 4 st2 state)
+    (NIL <state> 4)
+    ACL2 !>(fld st2)
+    NIL
+    ACL2 !>(fld st)
+    4
+    ACL2 !>
+
+  So far we have seen just one aliasing problem, i.e., between a free
+  stobj in a top-level form and a subsidiary updating
+  with-global-stobj form.  Another case is where the free stobj in a
+  top-level form is actually returned (we might say, updated) by that
+  form; in that case, any subsidiary with-global-stobj form is
+  problematic, even if it is read-only.  Here is an example.
+
+    (defun g2 (val st state)
+      (declare (xargs :stobjs (st state)))
+      (let ((st (update-fld val st)))
+        (let ((f (with-global-stobj st (fld st))))
+          (mv f (fld st) st state))))
+
+    (g2 nil st state)
+
+  As before, the definition is fine, but the ensuing top-level call is
+  not.  And as before, if we replace the top-level stobj occurrence
+  by one that is congruent to st, there is no error: (g2 5 st2
+  state).
+
+  Note that there is no aliasing problem when there is no update of the
+  stobj, either in the top-level form or in the subsidiary
+  with-global-stobj form.  The following are perfectly legal, for
+  example.
+
+    (defun g1 (st state)
+      (declare (xargs :stobjs (st state)))
+      (let ((f (with-global-stobj st (fld st))))
+        (mv f state (fld st))))
+
+    (g1 st state)
+
+  So far we have seen two similar error cases due to aliasing: both are
+  top-level calls involving a stobj occurrence that has an occurrence
+  below bound by with-global-stobj, where at least one of the two
+  occurrences updates the stobj.  Consider this: a top-level call
+  like (foo st state) could be viewed as grabbing st from the ACL2
+  state, hence could be viewed as being (with-global-stobj st (foo st
+  state)).  So we can think of the restrictions as being about nested
+  with-global-stobj calls, and that leads us to the final two cases.
+  Here is a summary of all the restrictions to prevent aliasing,
+  starting with the two discussed above about top-level evaluation,
+  and ending with the two new ones about nested with-global-stobj
+  calls.
+
+    * In a form u that is legal at the top-level, where u has a free
+      occurrence of the stobj st, there is no updating
+      with-global-stobj call that binds st and is invoked during
+      evaluation of u.
+    * In a form u that is legal at the top-level, where u returns the stobj
+      st, there is no with-global-stobj call that binds st and is
+      invoked during evaluation of u.
+    * In a legal form (with-global-stobj st u), there is no updating
+      with-global-stobj call that binds st and is invoked during
+      evaluation of u.
+    * In any form (with-global-stobj st lst u), there is no
+      with-global-stobj call that binds st and is invoked during
+      evaluation of u.
+
+  Our restrictions that prevent aliasing are syntactic ones, sufficient
+  to prevent the invocations described above.  They are implemented
+  by searching for calls of read-user-stobj-alist to identify
+  expansions of with-global-stobj calls, and by searing for calls of
+  write-user-stobj-alist to identify expansions of updating
+  with-global-stobj calls.
+
+  Finally, we note that the syntactic restrictions extend to [guard]s.
+  Consider again the function rd0 as defined above, and let's use it
+  in the guard of a function.
+
+    (defun rd0 (state)
+      (declare (xargs :stobjs state))
+      (with-global-stobj st (fld st)))
+
+    (defun call-rd0-in-guard (state)
+      (declare (xargs :stobjs state
+                      :guard (rd0 state))
+               (ignore state))
+      17)
+
+  Then as before, it is an error for a top-level form to update st and
+  also call a function that may lead to a with-global-stobj call that
+  binds st.
+
+    ACL2 !>(let ((st (update-fld 3 st)))
+             (mv st (call-rd0-in-guard state)))
+
+
+    ACL2 Error in TOP-LEVEL:  Illegal top-level form,
+    (LET ((ST (UPDATE-FLD 3 ST))) (LIST ST (CALL-RD0-IN-GUARD STATE))).
+    The stobj ST is returned by evaluation of that form, yet is bound by
+    a WITH-GLOBAL-STOBJ form, as the top-level form calls CALL-RD0-IN-GUARD,
+    which calls RD0, which makes a WITH-GLOBAL-STOBJ call that binds ST.
+    See :DOC with-global-stobj.
+
+    ACL2 !>
+
+
+Constrained Functions and Defattach
+
+  Consider the following constrained function introduction.
+
+    (encapsulate
+      (((crn0 state) => *))
+      (local (defun crn0 (state)
+               (declare (xargs :stobjs state))
+               (state-p state))))
+
+  If we try to attach rd0 (defined above) to crn0 we get an error, as
+  shown just below.  In short, this error says that since rd0 may
+  lead to a call of with-global-stobj that binds st, then with this
+  attachment, crn0 may lead to such a call; yet there is no record in
+  the [world] that crn0 may lead to such a call.
+
+    ACL2 !>(defattach crn0 rd0)
+
+
+    ACL2 Error in ( DEFATTACH CRN0 RD0):  The attachment of RD0 to CRN0
+    restricts stobjs bound by WITH-GLOBAL-STOBJ under calls of RD0, according
+    to the :GLOBAL-STOBJS keyword (default nil) in the signature introducing
+    CRN0.  But this restriction is violated for stobj ST:  the attempt
+    is to attach RD0, which makes a WITH-GLOBAL-STOBJ call that binds ST,
+    yet that stobj is not specified by the :GLOBAL-STOBJS keyword of CRN0.
+    See :DOC with-global-stobj.
+
+
+    Summary
+    Form:  ( DEFATTACH CRN0 RD0)
+    Rules: NIL
+    Time:  0.00 seconds (prove: 0.00, print: 0.00, other: 0.00)
+
+    ACL2 Error [Failure] in ( DEFATTACH CRN0 RD0):  See :DOC failure.
+
+    ******** FAILED ********
+    ACL2 !>
+
+  The solution is to note, in the signature of the constrained
+  function, that it may lead to a with-global-stobj call.  This is
+  accomplished by using the keyword, :GLOBAl-STOBJS, in the signature
+  of the function.  The value of that keyword is nil by default,
+  indicating that there is no such call.  Otherwise the value is a
+  cons of the form (r . w), where r and w are disjoint lists of
+  stobjs.  Their interpretation is as follows: w includes all stobjs
+  for which an attachment may have an updating with-global-stobj
+  call, and r includes all stobjs not in w for which an attachment
+  may have a with-global-stobj call.  Consider the following
+  modification of the [encapsulate] form above.
+
+    (encapsulate
+      (((crn1 state) => * :global-stobjs ((st) . nil)))
+      (local (defun crn1 (state)
+               (declare (xargs :stobjs state))
+               (state-p state))))
+
+  Then the form (defattach crn1 rd0) is legal: unlike crn0, crn1 has
+  specified that st may be bound by with-global-stobj in an
+  attachment.
+
+  The requirement is thus as follows.  Consider attachment of g to a
+  constrained function f, where g may lead to updating
+  with-global-stobj calls that bind stobjs w1, w2, ..., wk, and also
+  g may lead to with-global-stobj calls that bind, in addition to the
+  wi, stobjs r1, r2, ..., rn.  Then the signature of f must specify a
+  value (r . w) for the keyword :GLOBAL-STOBJS, where r and w are
+  lists of stobjs such that w includes all wi and the union of r and
+  w includes all ri.")
  (WITH-GUARD-CHECKING
   (GUARD ACL2-BUILT-INS)
   "Suppress or enable guard-checking for a form
